### Product Rule

- $xsin(x)$

$$(xsin(x))' = 1\cdot sin(x) + xcos(x) = sin(x) + cos(x)$$

---

- $x^2tan(x)$

$$(x^2tan(x))' = 2xtan(x) + x^2sec^2(x)$$

---

- $cos(x) + (x^2 + 1)sin(x)$

$$sin(x) + 2xsin(x) + (x^2+1)cos(x)$$

$$sin(x) + 2xsin(x) + x^2cos(x) + cos(x)$$

---

- $\sqrt{x}sec(x)$

$$(\sqrt{x}sec(x))' = \frac{1}{2\sqrt{x}}sec(x) + \sqrt{x}tan(x)sec(x)$$

---

- $xcotan(x)$

$$(xcotan(x))' = cotan(x) + x(-cosec^2(x))$$

$$= cotan(x) - xcosec^2(x)$$

---

- $x^2 + 3xtan(x)$

$$x^2 + 3xtan(x) = 2x + 3(xtan(x))' = 2x + 3 (tan(x) + xsec^2(x))$$

$$2x + 3tan(x) + 3xsec^2(x)$$

---

- $\frac{x + 1}{xsin(x)}$

$$\left(\frac{x + 1}{xsin(x)}\right)' = \frac{xsin(x) - (x+1)(xsin(x))'}{x^2sin^2(x)}$$

$$\frac{xsin(x) - (x+1)(sin(x) + xcos(x))}{x^2sin^2(x)}$$

$$\frac{xsin(x) - (xsin(x) + x^2cos(x) + sin(x) + xcos(x))}{x^2sin^2(x)}$$

$$\frac{xsin(x) - xsin(x) - x^2cos(x) - sin(x) - xcos(x)}{x^2sin^2(x)}$$

$$\frac{- x^2cos(x) - sin(x) - xcos(x)}{x^2sin^2(x)} = \frac{-xcos(x)(x + 1) - sin(x)}{x^2sin^2(x)}$$

---

- $(x^3 + \sqrt{x})cosec(x)$
