### Quotient Rule

- $\frac{x}{x^2+1}$

$$\left(\frac{x}{x^2+1}\right)' = \frac{1\cdot(x^2 + 1) - 1(2x)}{(x^2 + 1)^2} = \frac{x^2 -2x + 1}{(x^2 + 1)^2} = \frac{(x-1)^2}{(x^2 + 1)^2}$$

---

- $\frac{x^2 - 1}{x + 1}$

$$\left(\frac{x^2 - 1}{x + 1}\right)' = \frac{2x(x + 1) - (x^2-1)\cdot 1}{(x+1)^2} = \frac{2x^2 + 2x - x^2 + 1}{(x+1)^2}$$

$$\frac{x^2 + 2x + 1}{(x + 1)^2} = \frac{(x+1)^2}{(x+ 1)^2} = 1$$

---

- $\frac{3x^2 + 3}{5x - 3}$

$$\left(\frac{3x^2 + 3}{5x - 3}\right)' = \frac{6x(5x-3) - (3x^2 + 3)5}{(5x - 3)^2} = \frac{30x^2 -18x -(15x^2 + 3)}{(5x-3)^2}$$

$$= \frac{15x^2 - 18x + 3}{(5x - 3)^2} = \frac{3(5x^2 - 6x + 1)}{(5x - 3)^2}$$

---

- $\frac{\sqrt{x}}{x + 1}$

$$\left(\frac{\sqrt{x}}{x + 1}\right)' = \frac{\frac{1}{2\sqrt{x}}(x+ 1) - \sqrt{x}}{(x + 1)^2} = \frac{\frac{\sqrt{x}}{2x}(x+ 1) - \sqrt{x}}{(x+1)^2}= \frac{\frac{\sqrt{x}}{2} + \frac{\sqrt{x}}{2x} - \sqrt{x}}{(x+1)^2}$$

$$\frac{\frac{\sqrt{x} - x\sqrt{x}}{2x}}{(x+1) ^2} = \frac{\sqrt{x}(1 - x)}{2x(x+1)^2}$$

---

- $5x + \frac{x}{x-1}$

$$\left(5x + \frac{x}{x-1}\right)' = 5 + \frac{x-1 - x}{(x-1)^2} = 5 + \frac{-1}{(x-1)^2}$$

---

- $\sqrt{x} + \frac{3}{x^3 + 2}$

$$\left(\sqrt{x} + \frac{3}{x^3 + 2}\right)' = \frac{1}{2\sqrt{x}} + \frac{3(3x^2)}{(x^3 + 2)^2} = \frac{1}{2\sqrt{x}} + \frac{9x^2}{(x^3 + 2)^2}$$

---

- $\frac{\sqrt[3]{x} + x}{\sqrt{x}}$

$$\left(\frac{\sqrt[3]{x} + x}{\sqrt{x}}\right)' =  \frac{(\sqrt[3]{x} + x)'\sqrt{x} - (\sqrt[3]{x} + x)\frac{1}{2\sqrt{x}}}{(\sqrt{x})^2}$$

$$= \frac{\left(-\frac{1}{3\sqrt[3]{x^2}} + 1\right)\sqrt{x} - \frac{\sqrt[3]{x} + x}{2\sqrt{x}}}{x}$$

---

- $\frac{x + \sqrt[4]{x}}{x^2 + 3}$

$$\left(\frac{x + \sqrt[4]{x}}{x^2 + 3}\right)' = \frac{(x + \sqrt[4]{x})'\cdot(x^2 + 3) - (x+\sqrt[4]{x})\cdot(x^2 + 3)'}{(x^2 + 3)^2}$$

$$= \frac{\left(1 + \frac{1}{4\sqrt[4]{x^3}}\right)(x^2 + 3) - (x+\sqrt[4]{x})2x}{(x^2 + 3)^2}$$
