### Trigonometrics

1. Let $f(x) = sin(x)$. Calculate

- $f'(x)$

If $f(x) = sin(x) \Rightarrow f'(x) = cos(x)$

- $f'(\frac{\pi}{4}) = cos(\frac{\pi}{4}) = \frac{\sqrt{2}}{2}$

---

2. Find the tangent line to the graph $f(x) = sin(x)$ where $x = 0$

The angular coefficient can be found by $f'(x)$ which is $f'(x) = cos(x)$ , since we want the tangnet line equation at $x = 0$ we have $f'(0) = cos(0) = 1$ as the angular coefficient.

The line equation is $m = \frac{y - y_0}{x - x_0}$, where $m$ is the angular coefficient. So we have:

$m = 1$

$$1 = \frac{y - f(0)}{x - 0} = \frac{y}{x} \Rightarrow y = x$$

---

3. Let $f(x) = cos(x)$. Calculate:

- $f'(x) = -sin(x)$

- $f'(0) = 0$

- $f'(\frac{\pi}{3}) = -sin(\frac{\pi}{3}) = -\frac{\sqrt{3}}{2}$

- $f'(\frac{\pi}{4}) = -sin(\frac{\pi}{4}) = -\frac{\sqrt{2}}{2}$

---

4. Calculate $f'(x)$ being:

- $f(x) = tan(x)$

$$f(x) = tan(x) = \frac{sin(x)}{cos(x)} \Rightarrow f'(x) = \left(\frac{sin(x)}{cos(x)}\right)' $$

$$\left(\frac{sin(x)}{cos(x)}\right)'= \frac{cos(x)cos(x) - sin(x)(-sin(x))}{cos^2(x)} = \frac{cos^2(x) +sin^2}{cos^2(x)}$$

$$= \frac{1}{cos^2(x)} = sec^2(x)$$

Therefore $f'(x) = sec^2(x)$

---

- $f(x) = sec(x)$

$$f(x) = sec(x) = \frac{1}{cos(x)} \Rightarrow f'(x) = \left(\frac{1}{cos(x)}\right)' $$

$$\left(\frac{1}{cos(x)}\right)' = \frac{1(-sin(x))}{cos^2(x)} = \frac{-sin(x)}{cos(x)cos(x)} = -sec(x)tan(x)$$

Therefore $f'(x) = -sec(x)tan(x)$

---

5. Find the tangent line equation to the graph $f(x) = tan(x)$ where $x = 0$

$f(x) = tan(x) \Rightarrow f'(x) = sec^2(x)$

$m = f'(0) = sec^2(0) = 1$

Since the line equation is $m = \frac{y - y_0}{x - x_0}$

$$1 = \frac{y - f(0)}{x - x_0} = \frac{y - 0}{x - 0} = \frac{y}{x} \Rightarrow y = x$$

Therefore the tangent line at $x= 0$ is $y = x$.

---

6. Let $f(x) = cotan(x)$. Calculate:

- $f'(x)$

$$f'(x) = \left(\frac{1}{tan(x)}\right)' = \frac{tan(x)-sec^2(x)}{tan^2(x)} = \frac{tan}{tan^2(x)} - \frac{sec^2(x)}{tan^2(x)}$$

$$f'(x) = cotan(x) - \frac{\frac{1}{cos^2(x)}}{\frac{sen^2(x)}{cos^2(x)}} = cotan(x) - \frac{1}{cos^2(x)}\cdot \frac{cos^2(x)}{sen^2(x)}$$

$$= cotan(x) - \frac{1}{sen^2(x)} = cotan(x) - cossec^2(x)$$

- $f'(\frac{\pi}{4})$

$$f'\left(\frac{\pi}{4}\right) = cotan\left(\frac{\pi}{4}\right) - cossec^2\left(\frac{\pi}{4}\right) = 1- \left(\frac{2}{\sqrt{2}}\right)^2 = 1-2= -1$$

---

7. Let $g(x) = cossec(x)$. Calculate:

- $g'(x)$

$$g'(x) = \left(\frac{1}{sin(x)}\right)' = \frac{cos(x)}{sin^2(x)} = cotan(x)cossec(x)$$

- $g'(\frac{\pi}{4})$

$$g'\left(\frac{\pi}{4}\right) = cotan\left(\frac{\pi}{4}\right)cossec\left(\frac{\pi}{4}\right) = 1\cdot\frac{2}{\sqrt{2}} = 1\cdot \sqrt{2} = \sqrt{2}
