### Polynomials

$a) \lim_{x \to +\infty}\frac{1}{x^2} = 0$

---

$b) \lim_{x \to -\infty}\frac{1}{x^3} = 0$

---

$c) \lim_{x \to -\infty}5x + \frac{1}{x}+\frac{3}{x^2} = -\infty$

---

$d) \lim_{x \to +\infty}2-\frac{1}{x} =2$

---

$e) \lim_{x \to +\infty}\frac{2x + 1}{x+3}$

$$\lim_{x \to +\infty}\frac{2x + 1}{x+3} = \lim_{x \to +\infty}\frac{x(2 + \frac{1}{x})}{x(1 + \frac{3}{x})} = \lim_{x \to +\infty} \frac{2 + \frac{1}{x}}{1+\frac{3}{x}} = \frac{2}{1} = 2$$

---

$f) \lim_{x \to -\infty}\frac{2x+1}{x+3}$

$$\lim_{x \to -\infty}\frac{2x+1}{x+3} = \lim_{x \to -\infty}\frac{x(2+\frac{1}{x})}{x(1+\frac{3}{x})} = \lim_{x \to -\infty}\frac{2 + \frac{1}{x}}{1 + \frac{3}{x}} = \frac{2}{1} = 2$$

---

$g) \lim_{x \to -\infty}\frac{x^2 - 2x + 3}{3x^2 + x + 1}$

$$\lim_{x \to -\infty}\frac{x^2 - 2x + 3}{3x^2 + x + 1} = \lim_{x \to -\infty}\frac{x^2(1 - \frac{2}{x} + \frac{3}{x^2})}{x^2(3 + \frac{1}{x} + \frac{1}{x^2})} = \lim_{x \to -\infty}\frac{1 - \frac{2}{x}+\frac{3}{x^2}}{3 + \frac{1}{x} + \frac{1}{x^2}}$$

---

$h) \lim_{x \to +\infty}\frac{5x^4 - 2x + 1}{4x^4 + 3x + 2}$

$$\lim_{x \to +\infty}\frac{5x^4 - 2x + 1}{4x^4 + 3x + 2} = \lim_{x \to +\infty}\frac{x^4(5 - \frac{2}{x^3} + \frac{1}{x^4})}{x^4(4 + \frac{3}{x^3} + \frac{2}{x^4})} = \lim_{x \to +\infty}\frac{5-\frac{2}{x^3}+\frac{1}{x^4}}{4+\frac{3}{x^3}+\frac{2}{x^4}} = \frac{5}{4}$$

---

$i) \lim_{x \to +\infty}\frac{x}{x^2 + 3x + 1}$

$$\lim_{x \to +\infty}\frac{x}{x^2 + 3x + 1} = \lim_{x \to +\infty}\frac{x}{x(x + 3 + \frac{1}{x})} = \lim_{x \to +\infty}\frac{1}{x+3+\frac{1}{x}} = 0$$

---

$j) \lim_{x \to -\infty}\frac{2x^3+1}{x^4+2x+3}$

$$\lim_{x \to -\infty}\frac{2x^3+1}{x^4+2x+3}=\lim_{x \to -\infty} \frac{x^4(\frac{2}{x}+\frac{1}{x^4})}{x^4(1 + \frac{2}{x^3} + \frac{3}{x^4})} = \lim_{x \to -\infty}\frac{\frac{2}{x} + \frac{1}{x^4}}{1 + \frac{2}{x^3} + \frac{3}{x^4}} = \frac{0}{1}=0$$

---

$l)\lim_{x \to +\infty}\sqrt[3]{5+\frac{2}{x}} = \sqrt[3]{5}$

---

$m)\lim_{x \to -\infty}\sqrt[3]{\frac{x}{x^2 + 3}}$

$$\lim_{x \to -\infty}\sqrt[3]{\frac{x}{x^2 + 3}} = \lim_{x \to -\infty}\sqrt[3]{\frac{x}{x(x+3)}} = \lim_{x \to -\infty}\sqrt[3]{\frac{1}{x + 3}} = \sqrt[3]{0} = 0$$

---

$n) \lim_{x \to +\infty}\frac{\sqrt{x^2 + 1}}{3x+2}$

$$\lim_{x \to +\infty}\frac{\sqrt{x^2 + 1}}{3x+2} = \lim_{x \to +\infty}\sqrt{\frac{x^2 + 1}{(3x+2)^2}} = \lim_{x \to +\infty}\sqrt{\frac{x^2 + 1}{9x^2 + 12x + 4}}$$

$$\lim_{x \to +\infty}\sqrt{\frac{x^2(1 + \frac{1}{x^2})}{x^2(9 + \frac{12}{x} + \frac{4}{x^2})}} = \lim_{x \to +\infty}\sqrt{\frac{1 + \frac{1}{x^2}}{9 + \frac{12}{x} + \frac{4}{x^2}}} = \frac{1}{3}$$

---

$o) \lim_{x \to +\infty} \frac{\sqrt[3]{x^3 + 2x - 1}}{\sqrt{x^2 + x + 1}}$

$$\lim_{x \to +\infty} \frac{\sqrt[3]{x^3 + 2x - 1}}{\sqrt{x^2 + x + 1}} = \lim_{x \to +\infty}\frac{\sqrt[3]{x^3(1 + \frac{2}{x^2}-\frac{1}{x^3})}}{\sqrt{x^2(1 + \frac{1}{x} + \frac{1}{x^2})}} = \lim_{x \to +\infty}\frac{x\sqrt[3]{1 + \frac{1}{x^2}-\frac{1}{x^3}}}{x\sqrt{1 + \frac{1}{x} + \frac{1}{x^2}}}$$

$$ \lim_{x \to +\infty}\frac{\sqrt[3]{1 + \frac{1}{x^2} - \frac{1}{x^3}}}{\sqrt{1 + \frac{1}{x} + \frac{1}{x^2}}} = 1$$

---

$p)\lim_{x \to +\infty}\frac{\sqrt{x} + \sqrt[3]{x}}{x^2 + 3}$

$$\lim_{x \to +\infty}\frac{\sqrt{x} + \sqrt[3]{x}}{x^2 + 3} = \lim_{x \to +\infty}\frac{\sqrt{\frac{x^4}{x^3}} + \sqrt[3]{\frac{x^6}{x^5}}}{x^2 + 3} = \lim_{x \to +\infty}\frac{x^2\sqrt{\frac{1}{x^3}}+x^2\sqrt[3]{\frac{1}{x^5}}}{x^2 + 3}$$

$$\lim_{x \to +\infty}\frac{x^2\sqrt{\frac{1}{x^3}} + x^2\sqrt[3]{\frac{1}{x^5}}}{x^2(1 + \frac{3}{x^2})} = \lim_{x \to +\infty}\frac{\sqrt{\frac{1}{x^3}} + \sqrt[3]{\frac{1}{x^5}}}{1 + \frac{3}{x^2}} = 0$$

---

$q)\lim_{x \to +\infty}\frac{3}{\sqrt{x}} = 0$

---

$r)\lim_{x \to +\infty}\left(x-\sqrt{x^2 + 1}\right)$

$$\lim_{x \to +\infty}\left(x-\sqrt{x^2 + 1}\right)= \lim_{x \to +\infty}\frac{\left(x-\sqrt{x^2 - 1}\right)(x + \sqrt{x^2 + 1})}{x+\sqrt{x^2+1}} = \lim_{x \to +\infty}\frac{x^2-x^2+1}{x+\sqrt{x^2 + 1}}$$

$$\lim_{x \to +\infty}\frac{1}{x+ \sqrt{x^2+1}} = \lim_{x \to +\infty}\frac{1}{x+x\sqrt{1 + \frac{1}{x^2}}} = \lim_{x \to +\infty}\frac{1}{x(1 + \sqrt{1+\frac{1}{x^2}})} = 0$$

---

$s)\lim_{x \to +\infty}{\left(\sqrt{x+1}-\sqrt{x+3}\right)}$

$$\lim_{x \to +\infty}{\left(\sqrt{x+1}-\sqrt{x+3}\right)}=\lim_{x \to +\infty}\left(\sqrt{x+1}-\sqrt{x+3}\right)\frac{\left(\sqrt{x+1} + \sqrt{x+3}\right)}{\left(\sqrt{x+1} + \sqrt{x+3}\right)}$$

$$\lim_{x \to +\infty}\frac{x+1-x-3}{\sqrt{x+1}+\sqrt{x+3}} = \lim_{x \to +\infty}\frac{-2}{\sqrt{x+1}+\sqrt{x+3}} = 0$$